Correctness.v
@@ -12,19 +12,33 @@ Notation "T⟦ e ⟧ Σ " := (expr_to_term Σ e) (at level 40).
 
 Import InterpreterEnvList.
 
-Theorem expr_to_term_sound n ns ρ Σ1 Σ2 (Γ := []) (e : expr) (t : term) (v : val) :
-  Σ2 ;;; Γ |- T⟦indexify ns e⟧Σ1 ⇓ t ->
-  expr_eval n Σ1 ρ e = Ok v ->
-  t = T⟦from_val v⟧Σ1.
+Theorem expr_to_term_sound n ρ Σ1 Σ2 (Γ:=[]) (e : expr) (t : term) (v : val) :
+  Σ2 ;;; Γ |- T⟦e⟧Σ1 ⇓ t ->
+  expr_eval_i n Σ1 ρ e = Ok v ->
+  t = T⟦from_val_i v⟧Σ1.
 Proof.
-  induction e using expr_ind_case.
-  + (* eRel - since we expect only named variables, this case is trivial*)
-    intros HT He. simpl in *. destruct n; tryfalse.
+  revert dependent v.
+  revert dependent t.
+  revert dependent ρ.
+  revert dependent n.
+  induction e using expr_ind_case;intros n1 ρ t1 v.
+  + (* eRel*)
+    (*This case is trivial because we assume that we deal with closed terms by putting Γ = [] *)
+    intros HT He. simpl in *. destruct n1; tryfalse. autounfold with facts in *.
+    simpl in *.
+    destruct (lookup_i ρ n) eqn:Hlookup;tryfalse. simpl in He;inversion He;subst.
+    inversion HT;subst;simpl in *. inversion isdecl. inversion isdecl.
   + (* eVar *)
-    intros HT He. destruct n; tryfalse. simpl in *.
-    (* we need to relate [ρ] and [ns] *)
-    admit.
+    (* This case is trivial because we only consider terms with de Bruijn indices *)
+    intros HT He. destruct n1; tryfalse.
   + (* eLambda *)
-    intros HT He. destruct n; tryfalse. simpl in HT. simpl in He.
+    intros HT He. destruct n1; tryfalse.
+    autounfold with facts in *. simpl in HT. simpl in He.
     inversion He. simpl. inversion HT. subst.
+    destruct ρ.
+    * simpl. repeat f_equal. apply subst_env_i_empty.
+    * simpl.
+      destruct (n0 =? n).
+      ** f_equal.
+
 Admitted.
